src/versions/standard/Int63/Int63_standard.v
@@ -18,8 +18,8 @@
 (** Naive software representation of Int63. To improve. Anyway, if you
     want efficiency, rather use native-coq. **)
 
-Require Export Cyclic63.
-Require Export Ring63.
+(* Require Export Cyclic31. *)
+Require Export Ring31.
 Require Export Int63Native.
 Require Export Int63Op.
 Require Export Int63Axioms.
